src/tree/SearchTree.dfy
@@ -1,0 +1,573 @@
+include "../../src/tree/Tree.dfy"
+include "../../src/tree/TreeData.dfy"
+
+lemma {:verify true} idem(m:map<K,V>,k:K,v:V)
+  requires k in m && m[k]==v
+  ensures (m-{k})[k:=v]==m
+{}
+
+lemma {:verify true} idem2(m:map<K,V>,k:K,v:V)
+  requires k !in m
+  ensures (m[k:=v])-{k}==m
+{}
+
+lemma {:verify true} SubAddToAddSub(p: map<K, V>, q: map<K, V>, k: K)
+  requires k !in q
+  ensures p - {k} + q == p + q - {k}
+{}
+
+class SearchTree {
+  var tree: Tree;
+
+  function Repr(): set<object>
+    reads this, tree
+  {
+    tree.Repr()
+  }
+
+  predicate Valid()
+    reads this, tree, tree.Repr()
+  {
+    && tree.Valid()
+    && tree.SearchTree()
+  }
+
+  function Model(): map<K, V>
+    reads this, tree, Repr()
+    requires Valid()
+  {
+    tree.Model()
+  }
+
+  static function ModelRec(sk: tree<TNode>): map<K, V>
+    reads set x | x in elems(sk) :: x`key
+    reads set x | x in elems(sk) :: x`value
+  {
+    Tree.ModelRec(sk)
+  }
+
+  constructor()
+    ensures Valid()
+    ensures Model() == map[]
+    ensures forall x {:trigger x in Repr(), x in old(Repr())} | x in Repr() :: fresh(x)
+    ensures fresh(Repr())
+    ensures forall x | x in Repr() :: allocated(x)
+  {
+    tree := new Tree();
+  }
+
+  static method {:verify true} FindRec(node: TNode?, ghost sk: tree<TNode>, k: K) returns (found: TNode?)
+    requires Tree.ValidRec(node, sk)
+    requires Tree.SearchTreeRec(sk)
+
+    ensures Tree.ValidRec(node, sk)
+    ensures Tree.SearchTreeRec(sk)
+    ensures found == null <==> k !in Tree.ModelRec(sk)
+    ensures found != null ==>
+      && found.key == k
+      && found.value == Tree.ModelRec(sk)[k]
+      && found in elems(sk)
+
+    requires forall x | x in elems(sk) :: allocated(x)
+  {
+    if node == null {
+      found := null;
+      //assert found != null ==> found.key == k && found.value == Tree.ModelRec(sk)[k] && found in elems(sk);
+    } else {
+      assert elems(sk) == elems(sk.left) + {sk.data} + elems(sk.right);
+      if k == node.key {
+        found := node;
+        /*
+        assert
+          && found == null <==> k !in Tree.ModelRec(sk)
+        by {
+          reveal Tree.ModelRec();
+        }
+        assert found != null;
+        assert found.key == k && found.value == Tree.ModelRec(sk)[k] && found in elems(sk) by {
+          reveal Tree.ModelRec();
+        }
+        */
+      } else if node.key < k {
+        /*
+        assert k !in Tree.ModelRec(sk.left) by {
+          reveal Tree.ModelRec();
+          Tree.ModelLemmas(node, sk);
+        }
+        */
+        found := FindRec(node.right, sk.right, k);
+        //assert Tree.ValidRec(node, sk);
+        /*
+        assert
+          && found == null <==> k !in Tree.ModelRec(sk)
+        by {
+          reveal Tree.ModelRec();
+          Tree.ModelLemmas(node, sk);
+          if found != null {
+            assert k in Tree.ModelRec(sk.right);
+            assert k in Tree.ModelRec(sk.right).Keys;
+            Tree.ModelLemmas(node.right, sk.right);
+            assert Tree.ModelRec(sk.right).Keys == Tree.TreeKeys(sk.right);
+            calc == {
+              Tree.ModelRec(sk).Keys;
+              Tree.TreeKeys(sk);
+              Tree.TreeKeys(sk.left) + Tree.TreeKeys(sk.right) + {node.key};
+              Tree.TreeKeys(sk.left) + Tree.ModelRec(sk.right).Keys + {node.key};
+            }
+            assert k in Tree.ModelRec(sk).Keys;
+            assert k in Tree.ModelRec(sk);
+          } else {
+            assert k !in Tree.ModelRec(sk.right);
+            assert k !in Tree.ModelRec(sk.left);
+            assert node.key != k;
+            assert k !in Tree.ModelRec(sk);
+          }
+        }
+        */
+        /*
+        assert found != null ==> found.key == k && found.value == Tree.ModelRec(sk)[k] && found in elems(sk) by {
+          reveal Tree.ModelRec();
+        }
+        */
+      } else if k < node.key {
+        found := FindRec(node.left, sk.left, k);
+      } else {
+        assert false;
+      }
+    }
+    assert
+      && (found == null <==> k !in Tree.ModelRec(sk))
+      && (found != null ==> found.key == k && found.value == Tree.ModelRec(sk)[k] && found in elems(sk))
+    by {
+      reveal Tree.ModelRec();
+      Tree.ModelLemmas(node, sk);
+    }
+  }
+
+  method {:verify true} Find(k: K) returns (found: TNode?)
+    requires Valid()
+    ensures found == null <==> k !in Model()
+    ensures found != null ==>
+      && found.key == k
+      && found.value == Model()[k]
+      && found in elems(tree.skeleton)
+
+    requires forall x | x in Repr() :: allocated(x)
+  {
+    assert Repr() == elems(tree.skeleton);
+    found := FindRec(tree.root, tree.skeleton, k);
+  }
+
+  method {:verify true} Search(k: K) returns (b: bool)
+    requires Valid()
+    ensures b == (k in Model())
+
+    requires forall x | x in Repr() :: allocated(x)
+  {
+    var found := Find(k);
+    return found != null;
+  }
+
+  method {:verify true} Get(k: K) returns (v: V)
+    requires Valid()
+    requires k in Model()
+    ensures Model()[k] == v
+
+    requires forall x | x in Repr() :: allocated(x)
+  {
+    var found := Find(k);
+    return found.value;
+  }
+
+  static method {:verify true} InsertRec(node: TNode?, ghost sk: tree<TNode>, k: K, v: V)
+      returns (newNode: TNode, ghost newSk: tree<TNode>, ghost insertedNode: TNode)
+    modifies set x | x in elems(sk) :: x`left
+    modifies set x | x in elems(sk) :: x`right
+    modifies set x | x in elems(sk) :: x`value
+
+    requires Tree.ValidRec(node, sk)
+    requires Tree.SearchTreeRec(sk)
+
+    ensures Tree.ValidRec(newNode, newSk)
+    ensures Tree.SearchTreeRec(newSk)
+    ensures Tree.ModelRec(newSk) == old(Tree.ModelRec(sk))[k := v]
+
+    ensures elems(newSk) == elems(sk)+{insertedNode}
+    ensures insertedNode.key == k && insertedNode.value == v
+    ensures forall n | n in elems(sk) && old(n.key) != k ::
+      n.key == old(n.key) && n.value == old(n.value)
+
+    requires forall x | x in elems(sk) :: allocated(x)
+    ensures forall x {:trigger x in elems(newSk), x in old(elems(sk))} | x in elems(newSk) - old(elems(sk)) :: fresh(x)
+    ensures fresh(elems(newSk)-old(elems(sk)))
+    ensures forall x | x in elems(newSk) :: allocated(x)
+  {
+    if node == null {
+      newNode := new TNode(null, k, v, null);
+      newSk := Node(Empty, newNode, Empty);
+      insertedNode := newNode;
+      assert Tree.ModelRec(newSk) == old(Tree.ModelRec(sk))[k := v] by {
+        reveal Tree.ModelRec();
+      }
+    } else {
+      assert sk.data == node;
+      newNode := node;
+      if k == node.key {
+        node.value := v;
+        newSk := sk;
+        insertedNode := node;
+        assert Tree.ModelRec(newSk) == old(Tree.ModelRec(sk))[k := v] by {
+          reveal Tree.ModelRec();
+        }
+      } else if node.key < k {
+        ghost var newSkRight;
+        node.right, newSkRight, insertedNode := InsertRec(node.right, sk.right, k, v);
+        newSk := Node(sk.left, node, newSkRight);
+        assert Tree.ModelRec(newSk) == old(Tree.ModelRec(sk))[k := v] by {
+          reveal Tree.ModelRec();
+        }
+      } else if k < node.key {
+        ghost var oMMRight := Tree.ModelRec(sk.right);
+        ghost var oMMLeft := Tree.ModelRec(sk.left);
+        ghost var oMM := Tree.ModelRec(sk);
+        Tree.keysSearchTree(sk, k);
+        ghost var newSkLeft;
+        node.left, newSkLeft, insertedNode := InsertRec(node.left, sk.left, k, v);
+        newSk := Node(newSkLeft, node, sk.right);
+
+        assert Tree.ModelRec(newSk) == old(Tree.ModelRec(sk))[k := v] by {
+          reveal Tree.ModelRec();
+          assert node.key!=k;
+          assert node.key==old(node.key) && node.value==old(node.value);
+          assert node.key !in oMMLeft && node.key !in oMMRight && node.key !=k;
+
+          assert newSk.left==newSkLeft && newSk.right==sk.right && newSk.data==node;
+          assert Tree.ModelRec(newSk.left)==oMMLeft[k:=v];
+          assert Tree.ModelRec(newSk.right)==oMMRight;
+          assert oMM==(oMMLeft+oMMRight)[node.key:=node.value];
+          Tree.oldNewModelRecL(newSk, old(Tree.ModelRec(sk)), oMMLeft, oMMRight, node, k, v);
+        }
+      } else {
+        assert false;
+      }
+    }
+  }
+
+  method {:verify true} Insert(k: K, v: V)
+    modifies this, tree, Repr()
+    requires Valid()
+    ensures Valid()
+    ensures Model() == old(Model())[k := v]
+
+    requires forall x | x in Repr() :: allocated(x)
+    ensures forall x {:trigger x in Repr(), x in old(Repr())} | x in Repr() - old(Repr()) :: fresh(x)
+    ensures fresh(Repr()-old(Repr()))
+    ensures forall x | x in Repr() :: allocated(x)
+  {
+    ghost var z;
+    tree.root, tree.skeleton, z := InsertRec(tree.root, tree.skeleton, k, v);
+  }
+
+  static method {:verify true} RemoveMinRec(node: TNode, ghost sk: tree<TNode>)
+      returns (newNode: TNode?, ghost newSk: tree<TNode>, removedNode: TNode)
+    //decreases size(sk)
+    modifies elems(sk)
+
+    requires Tree.ValidRec(node, sk)
+    requires Tree.SearchTreeRec(sk)
+
+    ensures Tree.ValidRec(newNode, newSk)
+    ensures Tree.SearchTreeRec(newSk)
+
+    ensures removedNode in elems(sk)
+    ensures removedNode !in elems(newSk)
+    ensures removedNode.key == old(removedNode.key)
+    ensures removedNode.value == old(removedNode.value)
+    ensures elems(newSk) == elems(sk) - {removedNode}
+
+    ensures removedNode.key in old(Tree.ModelRec(sk))
+    ensures old(Tree.ModelRec(sk))[removedNode.key] == removedNode.value
+    ensures Tree.ModelRec(newSk) == old(Tree.ModelRec(sk)) - {removedNode.key}
+
+    ensures forall n | n in elems(sk) ::
+      n.key == old(n.key) && n.value == old(n.value)
+    ensures forall n | n in elems(newSk) ::
+      removedNode.key < n.key
+
+    requires forall x | x in elems(sk) :: allocated(x)
+    ensures forall x {:trigger x in elems(newSk), x in old(elems(sk))} | x in elems(newSk) - old(elems(sk)) :: fresh(x)
+    ensures fresh(elems(newSk)-old(elems(sk)))
+    ensures forall x | x in elems(newSk) :: allocated(x)
+  {
+    if node.left == null {
+      newNode := node.right;
+      newSk := sk.right;
+      removedNode := node;
+      assert
+        && removedNode.key in old(Tree.ModelRec(sk))
+        && old(Tree.ModelRec(sk))[removedNode.key] == removedNode.value
+        && Tree.ModelRec(newSk) == old(Tree.ModelRec(sk)) - {removedNode.key}
+      by {
+        reveal Tree.ModelRec();
+        calc == {
+          Tree.ModelRec(newSk);
+          old(Tree.ModelRec(sk.right));
+          old(Tree.ModelRec(sk.right)) + (map[removedNode.key := removedNode.value] - {removedNode.key});
+          {
+            assert removedNode.key !in old(Tree.ModelRec(sk.right)) by {
+              Tree.ModelLemmas(node, sk);
+            }
+          }
+          (old(Tree.ModelRec(sk.right)) + map[removedNode.key := removedNode.value]) - {removedNode.key};
+          { assert old(Tree.ModelRec(sk.left)) == map[]; }
+          (old(Tree.ModelRec(sk.left)) + old(Tree.ModelRec(sk.right)) + map[removedNode.key := removedNode.value]) - {removedNode.key};
+          old(Tree.ModelRec(sk)) - {removedNode.key};
+        }
+      }
+    } else {
+      Tree.ModelLemmas(node, sk);
+      newNode := node;
+      newSk := sk;
+      ghost var newSkLeft;
+      newNode.left, newSkLeft, removedNode := RemoveMinRec(newNode.left, newSk.left);
+      newSk := Node(newSkLeft, newNode, newSk.right);
+      assert
+        && removedNode.key in old(Tree.ModelRec(sk))
+        && old(Tree.ModelRec(sk))[removedNode.key] == removedNode.value
+        && Tree.ModelRec(newSk) == old(Tree.ModelRec(sk)) - {removedNode.key}
+      by {
+        reveal Tree.ModelRec();
+        assert removedNode.key !in old(Tree.ModelRec(sk.right));
+        calc == {
+          Tree.ModelRec(newSk);
+          Tree.ModelRec(newSk.left) + Tree.ModelRec(newSk.right) + map[newNode.key := newNode.value];
+          old(Tree.ModelRec(sk.left)) - {removedNode.key} + Tree.ModelRec(newSk.right) + map[newNode.key := newNode.value];
+          {
+            assert removedNode.key !in Tree.ModelRec(newSk.right);
+            SubAddToAddSub(old(Tree.ModelRec(sk.left)), Tree.ModelRec(newSk.right), removedNode.key);
+          }
+          old(Tree.ModelRec(sk.left)) + Tree.ModelRec(newSk.right) - {removedNode.key} + map[newNode.key := newNode.value];
+          {
+            assert removedNode.key != newNode.key;
+            SubAddToAddSub(Tree.ModelRec(newSk.right), map[newNode.key := newNode.value], removedNode.key);
+          }
+          old(Tree.ModelRec(sk.left)) + Tree.ModelRec(newSk.right) + map[newNode.key := newNode.value] - {removedNode.key};
+          old(Tree.ModelRec(sk)) - {removedNode.key};
+        }
+      }
+    }
+  }
+
+  static method {:verify true} RemoveRec(node: TNode?, ghost sk: tree<TNode>, k: K)
+      returns (newNode: TNode?, ghost newSk: tree<TNode>, ghost removedNode: TNode?)
+    modifies elems(sk)
+    requires Tree.ValidRec(node, sk)
+    requires Tree.SearchTreeRec(sk)
+    ensures Tree.ValidRec(newNode, newSk)
+    ensures Tree.SearchTreeRec(newSk)
+
+    ensures forall n | n in elems(sk) ::
+      n.key == old(n.key) && n.value == old(n.value)
+    ensures elems(newSk) == elems(sk) - {removedNode}
+    ensures removedNode != null ==>
+      && removedNode in elems(sk)
+      && removedNode !in elems(newSk)
+      && removedNode.key == k
+
+    ensures removedNode == null <==> k !in old(ModelRec(sk))
+    ensures removedNode != null ==>
+      && removedNode.key in old(Tree.ModelRec(sk))
+      && old(Tree.ModelRec(sk))[removedNode.key] == removedNode.value
+    ensures ModelRec(newSk) == old(ModelRec(sk)) - {k}
+
+    requires forall x | x in elems(sk) :: allocated(x)
+    ensures forall x {:trigger x in elems(newSk), x in old(elems(sk))} | x in elems(newSk) - old(elems(sk)) :: fresh(x)
+    ensures fresh(elems(newSk)-old(elems(sk)))
+    ensures forall x | x in elems(newSk) :: allocated(x)
+  {
+    if node == null {
+      newNode := node;
+      newSk := sk;
+      removedNode := null;
+      assert
+        && ModelRec(newSk) == old(ModelRec(sk)) - {k}
+        && (removedNode != null ==>
+          && removedNode.key in old(Tree.ModelRec(sk))
+          && old(Tree.ModelRec(sk))[removedNode.key] == removedNode.value
+          && ModelRec(newSk) == old(ModelRec(sk)) - {removedNode.key})
+        && (removedNode == null <==> k !in old(ModelRec(sk)))
+      by {
+        reveal Tree.ModelRec();
+      }
+    } else {
+      if node.key > k {
+        assert k !in Tree.ModelRec(sk.right) by {
+          assert k !in Tree.TreeKeys(sk.right);
+          Tree.ModelLemmas(node.right, sk.right);
+        }
+        newNode := node;
+        newSk := sk;
+        ghost var newSkLeft;
+        newNode.left, newSkLeft, removedNode := RemoveRec(newNode.left, newSk.left, k);
+        newSk := Node(newSkLeft, newNode, newSk.right);
+
+        assert
+          && ModelRec(newSk) == old(ModelRec(sk)) - {k}
+          && (removedNode != null ==>
+            && removedNode.key in old(Tree.ModelRec(sk))
+            && old(Tree.ModelRec(sk))[removedNode.key] == removedNode.value
+            && ModelRec(newSk) == old(ModelRec(sk)) - {removedNode.key})
+          && (removedNode == null <==> k !in old(ModelRec(sk)))
+        by {
+          reveal Tree.ModelRec();
+          assert k !in old(Tree.ModelRec(sk.right));
+          if removedNode != null {
+            calc == {
+              Tree.ModelRec(newSk);
+              Tree.ModelRec(newSk.left) + Tree.ModelRec(newSk.right) + map[newNode.key := newNode.value];
+              old(Tree.ModelRec(sk.left)) - {removedNode.key} + Tree.ModelRec(newSk.right) + map[newNode.key := newNode.value];
+              {
+                assert removedNode.key !in Tree.ModelRec(newSk.right);
+                SubAddToAddSub(old(Tree.ModelRec(sk.left)), Tree.ModelRec(newSk.right), removedNode.key);
+              }
+              old(Tree.ModelRec(sk.left)) + Tree.ModelRec(newSk.right) - {removedNode.key} + map[newNode.key := newNode.value];
+              {
+                assert removedNode.key != newNode.key;
+                SubAddToAddSub(Tree.ModelRec(newSk.right), map[newNode.key := newNode.value], removedNode.key);
+              }
+              old(Tree.ModelRec(sk.left)) + Tree.ModelRec(newSk.right) + map[newNode.key := newNode.value] - {removedNode.key};
+              old(Tree.ModelRec(sk)) - {removedNode.key};
+            }
+          }
+        }
+      } else {
+        newNode := node;
+        newSk := sk;
+
+        if k == newNode.key && newNode.right == null {
+          assert node.key !in ModelRec(sk.left) by {
+            Tree.ModelLemmas(node, sk);
+          }
+          assert elems(sk) == elems(newSk) == elems(newSk.left) + {newNode};
+          assert elems(sk) - {newNode} == elems(newSk) - {newNode} == elems(newSk.left);
+          removedNode := newNode;
+          newNode := newNode.left;
+          newSk := newSk.left;
+          assert Tree.ValidRec(node, sk);
+          assert elems(newSk) == elems(sk) - {removedNode};
+          assert
+            && ModelRec(newSk) == old(ModelRec(sk)) - {k}
+            && (removedNode != null ==>
+              && removedNode.key in old(Tree.ModelRec(sk))
+              && old(Tree.ModelRec(sk))[removedNode.key] == removedNode.value
+              && ModelRec(newSk) == old(ModelRec(sk)) - {removedNode.key})
+            && (removedNode == null <==> k !in old(ModelRec(sk)))
+          by {
+            reveal Tree.ModelRec();
+            calc == {
+              ModelRec(newSk);
+              old(ModelRec(sk.left));
+              old(ModelRec(sk.left)) + (map[node.key := node.value] - {k});
+              { assert node.key !in ModelRec(sk.left); }
+              old(ModelRec(sk.left)) + map[node.key := node.value] - {k};
+              { assert old(ModelRec(sk.right)) == map[]; }
+              old(ModelRec(sk.left) + ModelRec(sk.right) + map[node.key := node.value]) - {k};
+              old(ModelRec(sk)) - {k};
+            }
+          }
+          return;
+        }
+
+        if k != newNode.key {
+          assert k !in Tree.ModelRec(sk.left) by {
+            assert k !in Tree.TreeKeys(sk.left);
+            Tree.ModelLemmas(node.left, sk.left);
+          }
+          ghost var newSkRight;
+          newNode.right, newSkRight, removedNode := RemoveRec(newNode.right, newSk.right, k);
+          newSk := Node(newSk.left, newNode, newSkRight);
+          assert
+            && ModelRec(newSk) == old(ModelRec(sk)) - {k}
+            && (removedNode != null ==>
+              && removedNode.key in old(Tree.ModelRec(sk))
+              && old(Tree.ModelRec(sk))[removedNode.key] == removedNode.value
+              && ModelRec(newSk) == old(ModelRec(sk)) - {removedNode.key})
+            && (removedNode == null <==> k !in old(ModelRec(sk)))
+          by {
+            reveal Tree.ModelRec();
+            assert k !in old(Tree.ModelRec(sk.left));
+            if removedNode != null {
+              calc == {
+                Tree.ModelRec(newSk);
+                Tree.ModelRec(newSk.left) + Tree.ModelRec(newSk.right) + map[newNode.key := newNode.value];
+                Tree.ModelRec(newSk.left) + old(Tree.ModelRec(sk.right)) - {removedNode.key} + map[newNode.key := newNode.value];
+                {
+                  assert removedNode.key != newNode.key;
+                  SubAddToAddSub(old(Tree.ModelRec(sk.right)), map[newNode.key := newNode.value], removedNode.key);
+                }
+                Tree.ModelRec(newSk.left) + old(Tree.ModelRec(sk.right)) + map[newNode.key := newNode.value] - {removedNode.key};
+                old(Tree.ModelRec(sk)) - {removedNode.key};
+              }
+            }
+          }
+        } else {
+          assert newNode.right != null;
+          assert k !in ModelRec(sk.left) && k !in ModelRec(sk.right) by {
+            Tree.ModelLemmas(node, sk);
+          }
+          removedNode := newNode;
+          ghost var oldNewSkLeft := newSk.left;
+          var oldNewNodeLeft := newNode.left;
+          ghost var newSkRight;
+          var newNodeRight;
+          var minNode;
+          newNodeRight, newSkRight, minNode := RemoveMinRec(newNode.right, newSk.right);
+          newNode := minNode;
+          newNode.left := oldNewNodeLeft;
+          newNode.right := newNodeRight;
+          ghost var goodSk := Node(oldNewSkLeft, newNode, newSkRight);
+          newSk := goodSk;
+          assert
+            && ModelRec(newSk) == old(ModelRec(sk)) - {k}
+            && (removedNode != null ==>
+              && removedNode.key in old(Tree.ModelRec(sk))
+              && old(Tree.ModelRec(sk))[removedNode.key] == removedNode.value
+              && ModelRec(newSk) == old(ModelRec(sk)) - {removedNode.key})
+            && (removedNode == null <==> k !in old(ModelRec(sk)))
+          by {
+            reveal Tree.ModelRec();
+            calc == {
+              Tree.ModelRec(newSk);
+              Tree.ModelRec(newSk.left) + Tree.ModelRec(newSk.right) + map[newNode.key := newNode.value];
+              Tree.ModelRec(newSk.left) + old(Tree.ModelRec(sk.right)) - {minNode.key} + map[minNode.key := minNode.value];
+              { idem(old(Tree.ModelRec(sk.right)), minNode.key, minNode.value); }
+              Tree.ModelRec(newSk.left) + old(Tree.ModelRec(sk.right));
+              old(Tree.ModelRec(sk.left)) + old(Tree.ModelRec(sk.right));
+              old(Tree.ModelRec(sk.left)) + old(Tree.ModelRec(sk.right)) + map[];
+              { assert map[removedNode.key := removedNode.value] - {removedNode.key} == map[]; }
+              old(Tree.ModelRec(sk.left)) + old(Tree.ModelRec(sk.right)) + (map[removedNode.key := removedNode.value] - {removedNode.key});
+              { idem2(old(Tree.ModelRec(sk.left)) + old(Tree.ModelRec(sk.right)), removedNode.key, removedNode.value); }
+              old(Tree.ModelRec(sk.left)) + old(Tree.ModelRec(sk.right)) + map[removedNode.key := removedNode.value] - {removedNode.key};
+              old(Tree.ModelRec(sk)) - {removedNode.key};
+            }
+          }
+        }
+      }
+    }
+  }
+
+  method {:verify true} Remove(k: K)
+    modifies this, tree, Repr()
+    requires Valid()
+    ensures Valid()
+    ensures Model() == old(Model()) - {k}
+
+    requires forall x | x in Repr() :: allocated(x)
+    ensures forall x {:trigger x in Repr(), x in old(Repr())} | x in Repr() - old(Repr()) :: fresh(x)
+    ensures fresh(Repr()-old(Repr()))
+    ensures forall x | x in Repr() :: allocated(x)
+  {
+    ghost var z;
+    tree.root, tree.skeleton, z := RemoveRec(tree.root, tree.skeleton, k);
+  }
+}
